Date 18/07/2021



|      |  f   |  g   |  out |
| ---- | ---- | ---- | ---- |
|  0   |  0   |  1   |  0   |
|  1   |  1   |  0   |  1   |
|  2   |  1   |  1   |  1   |
|  3   |  2   |  1   |  2   |
|  4   |  3   |  2   |  3   |
|  6   |  5   |  3   |  5   |
|  7   |  8   |  5   |  8   |
|  8   |  13  |  8   |  13  |
|  9   |  21  |  13  |  21  |
|  10  |  34  |  21  |  34  |
|  11  |  55  |  34  |  55  |
|  12  |  89  |  55  |  89  |
|  13  | 144  |  89  | 144  |
|  14  | 233  | 144  | 233  |
|  15  | 377  | 233  | 377  |

Yes, the code `f = f + g;   g = f - g` make `g = f`
And you can also write this code
```java
public static int Fibonacci(int n) {
    if (n <= 1)
        return n;
    return f(n-1) + f(n-2);
}
```
Or another version
```cpp
int  Fibonacci(int& prev, int n) {
        if (n == 0) {
            prev = 1;
            return 0;
        }
        int prePrev;
        prev = Fibonacci(prePrev, n-1);
        return prePrev + prev;
    }
}
```
But the '&' is illegal in Java. So it is like this
```java
    public static void main(String[] args) {
        int[] j = new int[1];
        for (int i = 0; i < 15; i++) {
            StdOut.println(Fibonacci(j ,i));
        }
    }
    public static int Fibonacci(int[] prev, int n) {
        if (n == 0) {
            prev[0] = 1;
            return 0;
        }
        int[] prePrev = new int[1];
        prev[0] = Fibonacci(prePrev, n-1);
        return prePrev[0] + prev[0];
    }
```

